Intermediate/Typing.lean
@@ -8,13 +8,6 @@ open Lilac
 namespace Intermediate
 
 
-inductive VecTyping (J : A -> B -> Prop) : Vec A m -> Vec B m -> Prop
-| nil : VecTyping J .nil .nil
-| cons :
-  J a b ->
-  VecTyping J as bs ->
-  VecTyping J (a::as) (b::bs)
-
 def Query (G : List Global) (c : DataConst) (qs : Vec String m) (Ts : Vec Core.Ty m) : Prop :=
   VecTyping (lookup_ctor? G c · ·) qs Ts
 
